src/tls/MasterSecret.fst
@@ -1,63 +1,50 @@
 (* An experiment towards the PRF in KeySchedule, collapsing master and key derivation *)
 module MasterSecret (* : ST _ _ _ *)
 open FStar.HyperHeap
-
-(* tls_region is to be moved to TLSContants *)
-let tls_region = new_region root
-
+open TLSConstants
+open StreamAE
 module AE = StreamAE
 module MM = MonotoneMap
 module MR = FStar.Monotonic.RRef
 module HH = FStar.HyperHeap
+module N = Nonce
+module I = IdNonce
 
-type writer (ids:(AE.id * rid)) = w:AE.writer (fst ids){HH.extends (StreamAE.State.region w) (snd ids)}
-let ids = (AE.id * rid)
-
-let region_exists (r:rid) = MR.witnessed (fun h -> Map.contains h r)
+//We maintain ms_tab, a map from ids i, to w:StreamAE.writer i
+//such that, w's region is known to be a child region of the 
+//region associated with i's nonce
+let writer (i:AE.id) = w:AE.writer i{
+  N.registered (I.nonce_of_id i) (HH.parent w.region) /\ 
+  HH.disjoint (HH.parent w.region) tls_region
+}  
     
-let map_invariant (m:MM.map' ids writer) =
-  forall i r. 
-    let wopt = MM.sel m (i, r) in
-    is_Some wopt ==>
-    HH.disjoint r tls_region 
-    /\ region_exists (StreamAE.State.region (Some.v wopt))
+let ms_tab : MM.t tls_tables_region AE.id writer (fun x -> True) = 
+  MM.alloc #TLSConstants.tls_tables_region #AE.id #writer #(fun x -> True)
 
-  (* Failed attempt *)
-  (* (forall i1 i2. is_Some (m i1) /\ is_Some (m i2) /\ fst i1 = fst i2 ==> i1 = i2) *)
-  (* /\ (forall i. is_None (m i) ==> (forall j. fst i = fst j ==> is_None (m j))) *)
-
-let ms_tab : MM.t tls_region ids writer map_invariant = 
-  MM.alloc #tls_region #ids #writer #map_invariant
-
-assume val gcut: f:(unit -> GTot Type){f()} -> Tot unit
-assume val gadmit: f:(unit -> GTot Type) -> Tot (u:unit{f()})
-assume val witness_rid: r:rid -> ST unit
-  (requires (fun h -> True))
-  (ensures (fun h0 _ h1 -> 
-	      h0 = h1 /\
-	      Map.contains h0 r /\
-	      region_exists r))
-	      
 let derive (r:rid) (i:AE.id) 
   : ST (AE.writer i)
-       (requires (fun h -> disjoint r tls_region))
+       (requires (fun h -> 
+	   HH.disjoint r tls_region /\
+	   N.registered (I.nonce_of_id i) r))
        (ensures (fun h0 w h1 -> 
-	   HH.extends (StreamAE.State.region w) r 
-	   /\ modifies (Set.singleton tls_region) h0 h1 //modifies at most the tls region
-	   /\ modifies_rref tls_region !{HH.as_ref (MR.as_rref ms_tab)} h0 h1 //and within it, at most ms_tab
-	   /\ MR.witnessed (MM.contains ms_tab (i,r) w) //and the writer is witnessed to be in ms_tab
+       	   HH.disjoint r tls_region 
+	   /\ N.registered (I.nonce_of_id i) r
+	   /\ HH.parent w.region = r
+	   /\ modifies (Set.singleton tls_tables_region) h0 h1 //modifies at most the tls_tables region
+	   /\ modifies_rref tls_tables_region !{HH.as_ref (MR.as_rref ms_tab)} h0 h1 //and within it, at most ms_tab
+	   /\ MR.witnessed (MM.contains ms_tab i w) //and the writer is witnessed to be in ms_tab
 	   /\ (let old_ms = MR.m_sel h0 ms_tab in
 	      let new_ms = MR.m_sel h1 ms_tab in
  	       old_ms = new_ms //either ms_tab didn't change at all
-	       \/ (new_ms = MM.upd old_ms (i,r) w //or we just added w to it
-		  /\ (TLSInfo.authId i ==> MR.m_sel h1 (AE.ilog (StreamAE.State.log w)) = Seq.createEmpty))))) //and it is a fresh log
-  = recall_region tls_region;
-    let y = MM.lookup ms_tab (i, r) in
-    match y with 
+	       \/ (new_ms = MM.upd old_ms i w //or we just added w to it
+	   	  /\ (TLSInfo.authId i ==> MR.m_sel h1 (AE.ilog w.log) = Seq.createEmpty))))) //and it is a fresh log
+  = MR.m_recall ms_tab;
+    match MM.lookup ms_tab i with
     | None -> 
       let w = AE.gen r i in 
-      witness_rid (StreamAE.State.region w);
-      MM.extend ms_tab (i,r) w;
+      MM.extend ms_tab i w;
       w
     | Some w -> 
+      N.testify (I.nonce_of_id i) r;   // n i -> r
+      N.testify (I.nonce_of_id i) (HH.parent w.region); //n i -> HH.parent w.region ==> r=w.region
       w
