src/tls/StreamAE.fsti
@@ -17,6 +17,7 @@ open TLSInfo
 open StreamPlain
 open MonotoneSeq
 open FStar.Monotonic.RRef
+module HH = HyperHeap
 
 type id = i:id { pv_of_id i = TLS_1p3 }
 
@@ -104,7 +105,7 @@ type reader i = s:state i Reader
 
 let genPost (#i:id) parent h0 (w:writer i) h1 = 
                modifies Set.empty h0 h1 /\
-               extends w.region parent /\
+               HH.parent w.region = parent /\
                fresh_region w.region h0 h1 /\
 	       (authId i ==>
   		      (m_contains (ilog w.log) h1 /\
@@ -137,7 +138,7 @@ val genReader: parent:rid -> #i:id -> w:writer i -> ST (reader i)
   (ensures  (fun h0 (r:reader i) h1 ->
                modifies Set.empty h0 h1 /\
                r.log_region = w.region /\
-               extends (r.region) parent /\
+               HH.parent r.region = parent /\
                fresh_region r.region h0 h1 /\
                op_Equality #(log_ref w.region i) w.log r.log /\
 	       m_contains (ctr r.counter) h1 /\
